backup (proc)

process/processes.v
@@ -1,231 +1,115 @@
 From mathcomp Require Import all_ssreflect.
-From SST Require Import aux.unscoped aux.expressions type.global tree.global tree.local.
-Require Import List String Datatypes ZArith Relations Setoid Morphisms .
+From elpi.apps Require Import derive.std.
+From SST Require Import aux.unscoped aux.expressions type.global tree.global tree.local. 
+Require Import List String Datatypes ZArith Relations Setoid Morphisms.
 Open Scope list_scope.
 From mathcomp Require Import ssreflect.seq.
 Import ListNotations.
 From Paco Require Import paco.
 Require Import Coq.Init.Datatypes.
-Require Import Coq.Arith.PeanoNat.
+Require Import Coq.Arith.PeanoNat. 
+Require Import JMeq.
 
 Section process.
-(* lambda appr *) 
+
 
 Inductive process : Type := 
   | p_var : fin -> process
   | p_inact : process
   | p_send : part -> label -> expr -> process -> process
-  | p_recv : part -> list (prod label process) -> process 
+  | p_recv : part -> list label -> list process -> process 
   | p_ite : expr -> process -> process -> process 
   | p_rec : fin -> process -> process.
 
-
-Example simple_mu : process := 
-  p_rec 0 (p_send "Alice" 1 (e_val (vnat 100)) (p_var 0)).
+Section process_ind_ref.
+  Variable P : process -> Prop.
+  Hypothesis P_var : forall n, P (p_var n).
+  Hypothesis P_inact : P (p_inact).
+  Hypothesis P_send : forall pt lb ex pr, P pr -> P (p_send pt lb ex pr).
+  Hypothesis P_recv : forall pt lb pr llb llp, Forall P llp -> P (p_recv pt lb pr llb llp).
+  Hypothesis P_ite : forall e P1 P2, P P1 -> P P2 -> P (p_ite e P1 P2).
+  Hypothesis P_rec : forall n pr, P pr -> P (p_rec n pr).
   
-Example Pcomplex_mu : process := 
-  p_rec 0 (p_recv "Alice" [
-    (0, p_var 0);
-    (1, p_rec 1 (p_recv "Bob" [
-       (3, p_var 0);
-       (4, p_var 1);
-       (5, p_inact)
-    ]));
-    (2, p_inact)
-  ]).
-  
+  Fixpoint process_ind_ref p : P p.
+  Proof.
+    destruct p.
+    - apply (P_var n).
+    - apply (P_inact).
+    - apply (P_send s n e p (process_ind_ref p)).
+    - apply (P_recv).
+      - apply (process_ind_ref p). 
+      induction l as [ | c l IH].
+      clear process_ind_ref.
+      - intros. apply ForallR_nil.
+      - specialize(ForallR_cons P (fst c) (snd c) l); intros.
+        - generalize (process_ind_ref (snd c)). intros. 
+          specialize(H H0 IH); intros.
+          specialize(surjective_pairing c); intros.
+          replace c with (c.1, c.2). easy.
+    - apply (P_ite e p1 p2 (process_ind_ref p1) (process_ind_ref p2)).
+    - apply (P_rec n p (process_ind_ref p)). 
+  Qed.
+End process_ind_ref.
 
-CoFixpoint Tcomplex_mu : ltt := 
-  ltt_recv "Alice" [
-    (0, sbool, Tcomplex_mu);
-    (1, sbool, complex_mu_1);
-    (2, sbool, ltt_end)
-  ]
-  with complex_mu_1 : ltt :=
-    ltt_recv "Bob" [(3, sbool, Tcomplex_mu); (4, sbool, complex_mu_1); (5, sbool, ltt_end)].
 
-Example recursive_mu : process :=
-  p_rec 0 (p_send "A" 0 (e_val (vnat 1)) (
-    p_rec 1 (p_recv "B" [
-      (1, p_var 0); 
-      (2, p_send "C" 2 (e_val (vnat 2)) (p_var 1))
-    ])
-  )).
+Section process_ind_ref.
+  Variable P : process -> Prop.
+  Hypothesis P_var : forall n, P (p_var n).
+  Hypothesis P_inact : P (p_inact).
+  Hypothesis P_send : forall pt lb ex pr, P pr -> P (p_send pt lb ex pr).
+  Hypothesis P_recv : forall pt lb pr llbp, ForallR P llbp -> P (p_recv pt lb pr llbp).
+  Hypothesis P_ite : forall e P1 P2, P P1 -> P P2 -> P (p_ite e P1 P2).
+  Hypothesis P_rec : forall n pr, P pr -> P (p_rec n pr).
   
-Example subst_mu : process := 
-  p_rec 0 (p_recv "Alice" [
-    (0, p_var 0);
-    (1, p_recv "Bob" [
-       (3, p_var 0);
-       (4, p_var 15);
-       (5, p_var 16);
-       (6, p_rec 2 p_inact)
-    ]);
-    (2, p_inact)
-  ]).
-  
+  Fixpoint process_ind_ref p : P p.
+  Proof.
+    destruct p.
+    - apply (P_var n).
+    - apply (P_inact).
+    - apply (P_send s n e p (process_ind_ref p)).
+    - apply (P_recv).
+      - apply (process_ind_ref p). 
+      induction l as [ | c l IH].
+      clear process_ind_ref.
+      - intros. apply ForallR_nil.
+      - specialize(ForallR_cons P (fst c) (snd c) l); intros.
+        - generalize (process_ind_ref (snd c)). intros. 
+          specialize(H H0 IH); intros.
+          specialize(surjective_pairing c); intros.
+          replace c with (c.1, c.2). easy.
+    - apply (P_ite e p1 p2 (process_ind_ref p1) (process_ind_ref p2)).
+    - apply (P_rec n p (process_ind_ref p)). 
+  Qed.
+End process_ind_ref.
 
-Fixpoint fv (P : process) : list fin := 
-  match P with
-    | p_var x => [x]
-    | p_send p l e P' => fv P'
-    | p_recv p lis => 
-       let fix next xs :=
-         match xs with 
-          | (_,p)::ys => (fv p) ++ next ys
-          | _ => []
-         end
-       in next lis 
-    | p_ite e p q => (fv p) ++ (fv q)
-    | p_rec n p => 
-      let fix fil k xs :=
-        match xs with
-          | x::ys => if Nat.eqb x k then fil k ys else x::(fil k ys)
-          | _ => []
-        end
-      in fil n (fv p)
-    | _ => []
-   end.
-   
+
 Fixpoint vars (P : process) : list fin :=
   match P with
     | p_var x => [x]
     | p_send p l e P' => vars P'
-    | p_recv p lis => 
+    | p_recv p _ ct llbp => 
        let fix next xs :=
          match xs with 
-          | (_,p)::ys => (vars p) ++ next ys
+          | (_,p)::ys => vars p ++ next ys
           | [] => []
          end
-       in next lis 
-    | p_ite e p q => (fv p) ++ (fv q)
+       in next llbp ++ vars ct
+    | p_ite e p q => (vars p) ++ (vars q)
     | p_rec n p => n :: vars p
     | _ => []
   end.
-   
-Definition fresh_from_list (lis : list fin) : fin :=
-  match lis with 
-    | [] => 0
-    | _ => 
-      let fix max_lis xs :=
-        match xs with
-          | x::ys => max x (max_lis ys)
-          | _ => 0
-        end
-      in 1 + (max_lis lis)
-    end.
 
-Definition fresh (lis : list process) : fin := 
-  let fix max_lis xs :=
-    match xs with
-      | x::ys => max x (max_lis ys)
-      | _ => 0
-    end
-  in max_lis (list_map (fun x => (fresh_from_list (vars x))) lis).
 
 Fixpoint rename_force (from : fin) (to : fin) (P : process) : process := 
   match P with 
     | p_var x => if Nat.eqb x from then p_var to else p_var x
     | p_send p l e P' => p_send p l e (rename_force from to P')
-    | p_recv p lis => p_recv p (list_map (prod_map (fun x => x) (fun x => rename_force from to x)) lis)
+    | p_recv p lb ct llbp => p_recv p lb (rename_force from to ct) (list_map (fun x => (fst x, rename_force from to (snd x))) llbp)
     | p_ite e p1 p2 => p_ite e (rename_force from to p1) (rename_force from to p2)
     | p_rec x P' => if Nat.eqb from x then P else p_rec x (rename_force from to P')
     | _ => P
-  end.
+  end. 
 
-(* Takes outermost p_rec and renames that and all variables binded to it to a fresh one*)
-Definition rename_fresh (P : process) (avoid : list fin) : process := 
-  match P with 
-    | p_rec x P' => 
-        let fre := max (fresh [P']) (fresh_from_list avoid)
-        in p_rec fre (rename_force x fre P') 
-    | _ => P
-  end.
-
-
-Compute rename_fresh recursive_mu [2;3;4].
-
-(* when fresh variables are generated, overrides previous mappings of that variable (effectively deletes them, acknowledging different binder)*)
-Definition rename_pseudo_bruijn (P : process) (avoid : list fin) : process := 
-  let fix ren p av mp := 
-    match p with
-      | p_var x => 
-          let fix maps_using xs x := 
-            match xs with 
-              | (from,to)::ys => if Nat.eqb from x then to else maps_using ys x
-              | [] => x
-            end 
-          in p_var (maps_using mp x)
-      | p_send p l e P' => p_send p l e (ren P' av mp)
-      | p_recv p lis => p_recv p (list_map (prod_map (fun x => x) (fun x => ren x av mp)) lis)
-      | p_ite e p1 p2 => p_ite e (ren p1 av mp) (ren p2 av mp)
-      | p_rec x P' => 
-          let fre := fresh_from_list av
-          in p_rec fre (ren P' (fre::av) ((x,fre)::mp))
-      | _ => p
-    end
-  in ren P (avoid ++ (fv P)) [].
- 
-
-Compute rename_pseudo_bruijn recursive_mu [].
-Compute recursive_mu.
-
-Definition expr_eq_dec : forall (x y : expr), { x = y } + { x <> y }.
-Proof.
-decide equality.
-decide equality.
-decide equality. decide equality. decide equality. decide equality. decide equality. decide equality. decide equality.
-Defined.
-
-Definition balpha_equiv (P : process) (Q : process) : bool :=
-  let fix syntax_eq P1 P2 :=
-    match P1 with 
-    | p_var x =>
-        match P2 with 
-          | p_var y => (Nat.eqb x y)
-          | _ => false
-        end
-    | p_inact =>
-        match P2 with
-          | p_inact => true 
-          | _ => false
-        end 
-    | p_send p l e P' =>
-        match P2 with
-          | p_send q l' e' Q' => (eqb p q) && (Nat.eqb l l') && (expr_eq_dec e e') && (syntax_eq P' Q')
-          | _ => false 
-        end
-    | p_recv p lis =>
-        match P2 with
-          | p_recv q lis' => 
-            let fix all_true xs ys := 
-              match xs with
-                | (l,p')::xs' => 
-                  match ys with 
-                    | [] => false 
-                    | (l',q')::ys' => (Nat.eqb l l') && (syntax_eq p' q') && (all_true xs' ys')
-                  end
-                | [] => 
-                  match ys with
-                    | [] => true
-                    | _ => false
-                  end
-              end
-            in (eqb p q) && (all_true lis lis')
-          | _ => false
-        end
-    | p_ite e p1 p2 =>
-        match P2 with 
-          | p_ite e' q1 q2 => (expr_eq_dec e e') && (syntax_eq p1 q1) && (syntax_eq p2 q2)
-          | _ => false 
-        end
-    | p_rec x P' =>
-        match P2 with 
-          | p_rec y Q' => if Nat.eqb x y then syntax_eq P' Q' else false
-          | _ => false 
-        end
-   end
-  in syntax_eq (rename_pseudo_bruijn P (fv P ++ fv Q)) (rename_pseudo_bruijn Q (fv P ++ fv Q)).
 
 Definition fresh_in (x : fin) (P : process) : Prop :=
   let fix isin x lis :=
@@ -234,26 +118,169 @@ Definition fresh_in (x : fin) (P : process) : Prop :=
       | _ => True
     end
   in isin x (vars P).
-  
-Definition p_rename (from : fin) (to : fin) (P : process) (Q : process) : Prop := 
-  rename_force from to P = Q.
- 
-Inductive alphaP : relation process :=
-  | a_send : forall p l e P P', alphaP P P' -> alphaP (p_send p l e P) (p_send p l e P')
-  | a_recv : forall p xs ys, length xs = length ys -> List.Forall (fun u => (fst (fst u)) = (fst (snd u)) /\ alphaP (snd (fst u)) (snd (snd u))) (zip xs ys) -> alphaP (p_recv p xs) (p_recv p ys)
-  | a_ite  : forall e P1 P2 Q1 Q2, alphaP P1 Q1 -> alphaP P2 Q2 -> alphaP (p_ite e P1 P2) (p_ite e Q1 Q2)
-  | a_rec1  : forall x y P Q, fresh_in y (p_rec x P) -> p_rename x y P Q -> alphaP (p_rec x P) (p_rec y Q)
-  | a_rec2  : forall x P Q, alphaP P Q -> alphaP (p_rec x P) (p_rec x Q).
-  
-   
+
 Lemma freshness_in_rec : forall (x y : fin) (P : process), fresh_in y (p_rec x P) -> (y <> x).
 Proof.
   intros x y P.
   unfold fresh_in. unfold vars.
   easy.
 Qed.
+  
+Definition p_rename (from : fin) (to : fin) (P : process) (Q : process) : Prop := 
+  rename_force from to P = Q.
+  
+Section alphaP.
 
-Declare Instance Equivalence_alpha : Equivalence alphaP.
+ 
+Inductive alphaP : relation process :=
+  | a_inact : alphaP (p_inact) (p_inact)
+  | a_var : forall n, alphaP (p_var n) (p_var n)
+  | a_send : forall p l e P P', alphaP P P' -> alphaP (p_send p l e P) (p_send p l e P')
+  | a_recv : forall p llb xs ys lb x y, length llb = length xs -> length llb = length ys -> alphaP x y -> List.Forall2 alphaP xs ys -> alphaP (p_recv p lb x (zip llb xs)) (p_recv p lb y (zip llb ys))
+  | a_ite  : forall e P1 P2 Q1 Q2, alphaP P1 Q1 -> alphaP P2 Q2 -> alphaP (p_ite e P1 P2) (p_ite e Q1 Q2)
+  | a_recl  : forall x y P Q, fresh_in y (p_rec x P) -> p_rename x y P Q -> alphaP P Q -> alphaP (p_rec x P) (p_rec y Q)
+  | a_recr  : forall x y P Q, fresh_in x (p_rec y Q) -> p_rename y x Q P -> alphaP P Q -> alphaP (p_rec x P) (p_rec y Q)
+  | a_rec2  : forall x P Q, alphaP P Q -> alphaP (p_rec x P) (p_rec x Q).
+
+
+Definition Forall2_mono {X Y} {R T : X -> Y -> Prop} (HRT : forall x y, R x y -> T x y) :
+      forall l m, Forall2 R l m -> Forall2 T l m :=
+  fix loop l m h {struct h} :=
+    match h with
+    | Forall2_nil => Forall2_nil T
+    | Forall2_cons _ _ _ _ h1 h2 => Forall2_cons _ _ (HRT _ _ h1) (loop _ _ h2)
+    end.
+
+Section alphaP_ind_ref.
+  
+  Variable P : process -> process -> Prop.
+  Hypothesis P_inact : P p_inact p_inact.
+  Hypothesis P_var  : forall n, P (p_var n) (p_var n).
+  Hypothesis P_send : forall p l e P1 P2, P P1 P2 -> P (p_send p l e P1) (p_send p l e P2).
+  Hypothesis P_recv : forall p lb x y llb xs ys, length llb = length xs -> length llb = length ys -> P x y 
+                      -> List.Forall2 P xs ys -> P (p_recv p lb x (zip llb xs)) (p_recv p lb y (zip llb ys)).
+  Hypothesis P_ite  : forall e P1 P2 Q1 Q2, P P1 Q1 -> P P2 Q2 -> P (p_ite e P1 P2) (p_ite e Q1 Q2).
+  Hypothesis P_recl : forall x y P1 P2, fresh_in y (p_rec x P1) -> p_rename x y P1 P2 -> P P1 P2 -> P (p_rec x P1) (p_rec y P2).
+  Hypothesis P_recr : forall x y P1 P2, fresh_in x (p_rec y P2) -> p_rename y x P2 P1 -> P P1 P2 -> P (p_rec x P1) (p_rec y P2).
+  Hypothesis P_recn : forall x P1 P2, P P1 P2 -> P (p_rec x P1) (p_rec x P2). 
+
+  Fixpoint alphaP_ind_ref (P1 P2 : process) (a : alphaP P1 P2) {struct a} : P P1 P2 :=
+    match a with 
+      | a_inact => P_inact
+      | a_var n => P_var n
+      | a_send p l e P1 P2 H => P_send p l e P1 P2 (alphaP_ind_ref P1 P2 H) 
+      | a_recv p llb xs ys lb x y Hlx Hly Ha La => P_recv p lb x y llb xs ys Hlx Hly (alphaP_ind_ref x y Ha) (Forall2_mono alphaP_ind_ref xs ys La)
+      | a_ite e P1 P2 Q1 Q2 H1 H2 => P_ite e P1 P2 Q1 Q2 (alphaP_ind_ref P1 Q1 H1) (alphaP_ind_ref P2 Q2 H2)
+      | a_recl x y P1 P2 Hfy Hr Ha => P_recl x y P1 P2 Hfy Hr (alphaP_ind_ref P1 P2 Ha)
+      | a_recr x y P1 P2 Hfy Hr Ha => P_recr x y P1 P2 Hfy Hr (alphaP_ind_ref P1 P2 Ha)
+      | a_rec2 x P1 P2 Ha => P_recn x P1 P2 (alphaP_ind_ref P1 P2 Ha)
+    end.
+
+End alphaP_ind_ref.
+
+
+Lemma list_fst_snd_len {A B: Type} : forall (lis : list (A*B)), length (list_map fst lis) = length (list_map snd lis).
+Proof.
+  intros.
+  induction lis.
+  easy.
+  simpl. 
+  replace (length (list_map fst lis)) with (length (list_map snd lis)).
+  easy.
+Qed.
+
+Lemma unzip_zip {A B : Type} : forall (lis : list (A*B)), lis = zip (list_map fst lis) (list_map snd lis).
+Proof.
+  intros.
+  induction lis.
+  - easy.
+  - simpl. replace lis with (zip (list_map fst lis) (list_map snd lis)) at 1.
+    specialize(surjective_pairing a); intros. 
+    replace a with (a.1,a.2). easy.
+Qed.
+
+Lemma refl_alphaP : forall P, alphaP P P.
+Proof.
+  intros. 
+  induction P using process_ind_ref.
+  - specialize(a_var n); intros; try easy.
+  - specialize(a_inact); intros; try easy.
+  - specialize(a_send pt lb ex P P IHP); intros; try easy.
+  - specialize(a_recv); intros.
+    induction llbp.
+      - specialize(H0 pt [] [] [] lb P P); intros. 
+        specialize(H0 (Logic.eq_refl (length [])) (Logic.eq_refl (length [])) IHP); intros.
+        assert(Forall2 alphaP [] []). { easy. }
+        specialize(H0 H1); intros; try easy.
+        specialize(H0 pt (list_map fst (a::llbp)) (list_map snd (a::llbp)) (list_map snd (a::llbp)) lb P P); intros.
+        specialize((list_fst_snd_len (a::llbp))); intros.
+        specialize(H0 H1 H1 IHP); intros.
+        specialize(unzip_zip (a::llbp)); intros. 
+        replace (zip (list_map fst (a :: llbp)) (list_map snd (a :: llbp))) with (a::llbp) in H0.
+        clear H1 H2.
+        
+        
+        
+        specialize( IHP); intros.
+      -  
+
+Lemma sym_alphaP : forall P Q, alphaP P Q -> alphaP Q P.
+Proof.
+  intros.
+  induction H using alphaP_ind_ref; intros; try easy.
+  - specialize(a_inact); intros. easy.
+  - specialize(a_var n); intros. easy.
+  - specialize(a_send p l e P2 P1 IHalphaP); intros. easy.
+  - assert(Forall2 alphaP ys xs).
+    {
+      specialize(Forall2_flip H1); intros.
+      simpl in H2. easy.
+    }
+    specialize(a_recv p llb ys xs lb y x H0 H IHalphaP H2); intros. easy.
+  - specialize(a_ite e Q1 Q2 P1 P2 IHalphaP IHalphaP0); intros. easy.
+  - specialize(a_recr y x P2 P1 H H0 IHalphaP); intros. easy.
+  - specialize(a_recl y x P2 P1 H H0 IHalphaP); intros. easy.
+  - specialize(a_rec2 x P2 P1 IHalphaP); intros. easy.
+Qed.
+
+
+
+Lemma alphaP_inv_send : forall P P' p l e, alphaP P (p_send p l e P') 
+  -> exists Q, P = p_send p l e Q /\ alphaP Q P'.
+Proof.
+  intros. inversion H. exists P'. split; try easy. apply (a_refl P').
+  exists P0. easy. 
+Qed.
+
+Lemma zipeq {A : Type} : forall (x y : A) (xs : list A), In (x,y) (zip xs xs) -> x = y.
+  intros x y xs.
+  induction xs.
+  easy. 
+  simpl. 
+  intros. destruct H. 
+  specialize(pair_equal_spec a x a y); intros. destruct H0. specialize(H0 H); intros.
+  destruct H0. subst. easy.
+  specialize(IHxs H); intros.
+  easy.
+Qed.
+  
+Lemma alphaP_cong_recv : forall P p lb x llb xs, alphaP P (p_recv p lb x llb xs) 
+  -> exists y ys, P = p_recv p lb y llb ys /\ alphaP x y /\ List.Forall (fun u => alphaP (fst u) (snd u)) (zip xs ys).
+Proof.
+  intros. inversion H. exists x. exists xs. 
+  split. easy. split. apply (a_refl x). 
+  apply Forall_forall. intros.
+  specialize(surjective_pairing x0); intros.
+  specialize(zipeq x0.1 x0.2 xs); intros.
+  replace (x0.1,x0.2) with x0 in H4.
+  specialize(H4 H2); intros. specialize(a_refl x0.1); intros.
+  replace x0.1 with x0.2 in *. easy.
+  exists x0. exists xs0.
+  split. easy. split. 
+  admit.
+  admit.
+Admitted.
+     
 
 Inductive multi {X : Type} (R : relation X) : relation X :=
   | multi_refl : forall (x : X), multi R x x
@@ -261,86 +288,18 @@ Inductive multi {X : Type} (R : relation X) : relation X :=
 
 Definition alpha_multistep : relation process := multi alphaP.
 
-Definition al1 := p_rec 0 (p_rec 1 (p_recv "Alice " [(1, p_var 0); (2, p_var 1)])).
-Definition al2 := p_rec 1 (p_rec 0 (p_recv "Alice " [(1, p_var 1); (2, p_var 0)])).
-Definition al3 := p_rec 20 (p_rec 13 (p_recv "Alice " [(1, p_var 20); (2, p_var 13)])).
-Definition al4 := p_rec 0 (p_rec 1 (p_recv "Alice " [(1, p_var 1); (2, p_var 1)])).
-
-Compute balpha_equiv al1 al2.
-Compute balpha_equiv al1 al4.
-Compute rename_pseudo_bruijn (p_rec 20 (p_rec 13 (p_var 20))) [].
-
-(* Example t : 2 <> 3.
-Proof.
-  simpl. easy. *)
-(*
-Lemma stronger_multi {X : Type} (R : relation X) : forall (x y z : X), multi R x y -> multi R y z -> multi R x z.
-Proof.
-  intros x y z.
-   *)
-  
-
-Example al1_al3 : alpha_multistep al1 al3. 
-Proof.
-  unfold al1, al3.
-  unfold alpha_multistep.
-  apply multi_step with 
-  (y := (p_rec 20 (p_rec 1 (p_recv "Alice " [(1, p_var 20); (2, p_var 1)])))).
-  apply a_rec1. 
-  - unfold fresh_in. simpl. easy.
-  - unfold p_rename. unfold rename_force. simpl. easy.
-  
-  apply multi_step with 
-  (y := (p_rec 20 (p_rec 13 (p_recv "Alice " [(1, p_var 20); (2, p_var 13)])))).
-  apply a_rec2. apply a_rec1. 
-  - unfold fresh_in. simpl. easy.
-  - unfold p_rename; unfold rename_force. simpl. easy.
-  
-  apply multi_refl.
-  
-Qed.
-
-Example al3_al2 : alpha_multistep al3 al2. 
-Proof.
-  unfold al3, al2.
-  unfold alpha_multistep.
-  apply multi_step with 
-  (y := (p_rec 1 (p_rec 13 (p_recv "Alice " [(1, p_var 1); (2, p_var 13)])))).
-  apply a_rec1. 
-  - unfold fresh_in. simpl. easy.
-  - unfold p_rename. unfold rename_force. simpl. easy.
-  
-  apply multi_step with 
-  (y := (p_rec 1 (p_rec 0 (p_recv "Alice " [(1, p_var 1); (2, p_var 0)])))).
-  apply a_rec2. apply a_rec1. 
-  - unfold fresh_in. simpl. easy.
-  - unfold p_rename; unfold rename_force. simpl. easy.
-  
-  apply multi_refl.
-  
-Qed.
+End alphaP.
 
 Lemma transitive_multi {X : Type} : forall (R : relation X) (x y z : X), multi R x y -> multi R y z -> multi R x z.
 Proof.
   intros R x y z H.
   revert z.
-  
-(*   inversion H. subst.
-  easy. subst. inversion H0. subst. easy. subst. *)
   induction H; intros. easy.
   specialize(IHmulti z0 H1).
   specialize(@multi_step X R); intros.
   apply H2 with (y := y). easy. easy.
 Qed.
 
-Example al1_al2 : alpha_multistep al1 al2.
-Proof. 
-  unfold al1, al2.
-  apply transitive_multi with 
-  (y := al3).
-  apply al1_al3.
-  apply al3_al2.
-Qed.
 
 Definition quaternary_relation (A : Type) : Type := A -> A -> A -> A -> Prop.
 
@@ -353,25 +312,27 @@ Inductive substitutionP : quaternary_relation process :=
   | sub_var_not  : forall P x y, x <> y -> substitutionP (p_var x) P (p_var y) (p_var y)
   | sub_inact    : forall P x, substitutionP (p_var x) P (p_inact) (p_inact)
   | sub_send     : forall P x pt l e P' Q', substitutionP (p_var x) P P' Q' -> substitutionP (p_var x) P (p_send pt l e P') (p_send pt l e Q')
-  | sub_recv     : forall P x pt xs ys, length xs = length ys -> List.Forall (fun u => (fst (fst u)) = (fst (snd u)) /\ substitutionP (p_var x) P (snd (fst u)) (snd (snd u))) (zip xs ys) -> substitutionP (p_var x) P (p_recv pt xs) (p_recv pt ys)
- | sub_ite       : forall P x e P1 P2 Q1 Q2, substitutionP (p_var x) P P1 Q1 -> substitutionP (p_var x) P P2 Q2 -> substitutionP (p_var x) P (p_ite e P1 P2) (p_ite e Q1 Q2)
- | sub_rec       : forall P x y P' Q', x <> y -> fresh_in y P -> substitutionP (p_var x) P P' Q' -> substitutionP (p_var x) P (p_rec y P') (p_rec y Q')
- | sub_alpha     : forall P x P1 P2 Q, alphaP P1 P2 -> substitutionP (p_var x) P P1 Q -> substitutionP (p_var x) P P2 Q.
+  | sub_recv     : forall P x pt lb ct1 ct2 llb xs ys, length xs = length ys -> substitutionP (p_var x) P ct1 ct2 ->
+  List.Forall (fun u => substitutionP (p_var x) P (fst u) (snd u)) (zip xs ys) -> substitutionP (p_var x) P (p_recv pt lb ct1 llb xs) (p_recv pt lb ct2 llb ys)
+  | sub_ite       : forall P x e P1 P2 Q1 Q2, substitutionP (p_var x) P P1 Q1 -> substitutionP (p_var x) P P2 Q2 -> substitutionP (p_var x) P (p_ite e P1 P2) (p_ite e Q1 Q2)
+  | sub_rec       : forall P x y P' Q', x <> y -> fresh_in y P -> substitutionP (p_var x) P P' Q' -> substitutionP (p_var x) P (p_rec y P') (p_rec y Q')
+  | sub_alpha     : forall P x P1 P2 Q, alpha_multistep P1 P2 -> substitutionP (p_var x) P P1 Q -> substitutionP (p_var x) P P2 Q.
  (* | sub_alpha     : forall P x P' Q1 Q2, substitutionP (p_var x) P P' Q1 -> alphaP Q1 Q2 -> substitutionP (p_var x) P P' Q2. *)
   
 
-Example alpha_subst : substitutionP (p_var 0) (p_var 1) (p_rec 1 (p_ite (e_var 100) (p_var 0) (p_var 1))) (p_rec 2 (p_ite (e_var 100) (p_var 1) (p_var 2))).
+(* Example alpha_subst : substitutionP (p_var 0) (p_var 1) (p_rec 1 (p_ite (e_var 100) (p_var 0) (p_var 1))) (p_rec 2 (p_ite (e_var 100) (p_var 1) (p_var 2))).
 Proof.
   apply sub_alpha with 
   (P1 := (p_rec 2 (p_ite (e_var 100) (p_var 0) (p_var 2)))).
-  - apply a_rec1. unfold fresh_in. simpl. easy.
+  - apply a_recl. unfold fresh_in. simpl. easy.
   - unfold p_rename. unfold rename_force. simpl. easy.
   apply sub_rec. 
   - easy.
   - unfold fresh_in. simpl. easy.
   repeat constructor. easy.
 Qed.
-
+ *)
+(* 
 Inductive scongP : relation process := 
   | sc_subst    : forall P x Q, substitutionP (p_var x) (p_rec x P) P Q -> scongP (p_rec x P) Q
   | sc_alpha    : forall P Q, alphaP P Q -> scongP P Q
@@ -443,7 +404,8 @@ Definition subst_expr_proc (p : process) (l : label) (e : expr) : (option proces
     | _ => None
   end.
 
+
+ *)
+
 End process.
-
-
 
