process/box.v
@@ -1,0 +1,55 @@
+
+
+Inductive Box : Type := 
+  | Simple : Box
+  | InBox : list Box -> Box.
+
+Inductive Rel : relation Box := 
+  | R_refl : forall B, Rel B B
+  | R_box  : forall A B, List.Forall2 Rel A B -> Rel (InBox A) (InBox B).
+
+Section Rel_ref.
+  Variable P : Box -> Box -> Prop.
+  Variable P_list : list Box -> list Box -> Prop.
+  Variable P_nil : P_list [] [].
+  Variable P_cons : forall t1 t2 l1 l2, P t1 t2 -> P_list l1 l2 -> P_list (t1 :: l1) (t2 :: l2).
+  Variable P_refl : forall B, P B B.
+  Variable P_box  : forall A B, P_list A B -> P (InBox A) (InBox B).
+  
+  Fixpoint Rel_ref (B1 B2 : Box) (a : Rel B1 B2) {struct a}: P B1 B2 :=
+    let fix go_list (l1 l2 : list Box) (H : List.Forall2 Rel l1 l2) {struct H} : P_list l1 l2 :=
+      match H with
+        | Forall2_nil  =>  P_nil
+        | @Forall2_cons _ _ _ x y xr yr H1 H2 => P_cons x y xr yr (Rel_ref x y H1) (go_list xr yr H2)
+      end
+    in 
+    match a with
+      | R_refl B    => P_refl B
+      | R_box A B H => P_box A B (go_list A B H)
+    end.
+
+End Rel_ref.
+
+
+Definition Forall2_mono {X Y} {R T : X -> Y -> Prop} (HRT : forall x y, R x y -> T x y) :
+      forall l m, Forall2 R l m -> Forall2 T l m :=
+  fix loop l m h {struct h} :=
+    match h with
+    | Forall2_nil => Forall2_nil T
+    | Forall2_cons _ _ _ _ h1 h2 => Forall2_cons _ _ (HRT _ _ h1) (loop _ _ h2)
+    end.
+
+Section Rel_ind_ref.
+  Variable P : Box -> Box -> Prop.
+  Variable P_refl : forall B, P B B.
+  Variable P_box  : forall A B, Forall2 Rel A B -> Forall2 P A B -> P (InBox A) (InBox B).  
+  
+  Compute (List.Forall2_cons).
+  Compute (List.Forall_cons).
+
+  Fixpoint Rel_ind_ref (B1 B2 : Box) (a : Rel B1 B2) {struct a} : P B1 B2 := 
+    match a with
+    | R_refl B => P_refl B
+    | R_box A B H => P_box A B H (Forall2_mono Rel_ind_ref _ _ H)
+    end.
+End Rel_ind_ref.
