process/dump.v
@@ -1,0 +1,260 @@
+
+
+(* 
+Example simple_mu : process := 
+  p_rec 0 (p_send "Alice" 1 (e_val (vnat 100)) (p_var 0)).
+  
+Example Pcomplex_mu : process := 
+  p_rec 0 (p_recv "Alice" [
+    (0, p_var 0);
+    (1, p_rec 1 (p_recv "Bob" [
+       (3, p_var 0);
+       (4, p_var 1);
+       (5, p_inact)
+    ]));
+    (2, p_inact)
+  ]).
+  
+
+CoFixpoint Tcomplex_mu : ltt := 
+  ltt_recv "Alice" [
+    (0, sbool, Tcomplex_mu);
+    (1, sbool, complex_mu_1);
+    (2, sbool, ltt_end)
+  ]
+  with complex_mu_1 : ltt :=
+    ltt_recv "Bob" [(3, sbool, Tcomplex_mu); (4, sbool, complex_mu_1); (5, sbool, ltt_end)].
+
+Example recursive_mu : process :=
+  p_rec 0 (p_send "A" 0 (e_val (vnat 1)) (
+    p_rec 1 (p_recv "B" [
+      (1, p_var 0); 
+      (2, p_send "C" 2 (e_val (vnat 2)) (p_var 1))
+    ])
+  )).
+  
+Example subst_mu : process := 
+  p_rec 0 (p_recv "Alice" [
+    (0, p_var 0);
+    (1, p_recv "Bob" [
+       (3, p_var 0);
+       (4, p_var 15);
+       (5, p_var 16);
+       (6, p_rec 2 p_inact)
+    ]);
+    (2, p_inact)
+  ]).
+   *)
+(* 
+Fixpoint fv (P : process) : list fin := 
+  match P with
+    | p_var x => [x]
+    | p_send p l e P' => fv P'
+    | p_recv p lis => 
+       let fix next xs :=
+         match xs with 
+          | (_,p)::ys => (fv p) ++ next ys
+          | _ => []
+         end
+       in next lis 
+    | p_ite e p q => (fv p) ++ (fv q)
+    | p_rec n p => 
+      let fix fil k xs :=
+        match xs with
+          | x::ys => if Nat.eqb x k then fil k ys else x::(fil k ys)
+          | _ => []
+        end
+      in fil n (fv p)
+    | _ => []
+   end.
+    *)
+    
+    
+    
+(* 
+Definition fresh_from_list (lis : list fin) : fin :=
+  match lis with 
+    | [] => 0
+    | _ => 
+      let fix max_lis xs :=
+        match xs with
+          | x::ys => max x (max_lis ys)
+          | _ => 0
+        end
+      in 1 + (max_lis lis)
+    end.
+
+Definition fresh (lis : list process) : fin := 
+  let fix max_lis xs :=
+    match xs with
+      | x::ys => max x (max_lis ys)
+      | _ => 0
+    end
+  in max_lis (list_map (fun x => (fresh_from_list (vars x))) lis). *)
+  
+  
+(* Takes outermost p_rec and renames that and all variables binded to it to a fresh one*)
+Definition rename_fresh (P : process) (avoid : list fin) : process := 
+  match P with 
+    | p_rec x P' => 
+        let fre := max (fresh [P']) (fresh_from_list avoid)
+        in p_rec fre (rename_force x fre P') 
+    | _ => P
+  end.
+
+
+Compute rename_fresh recursive_mu [2;3;4].
+
+(* when fresh variables are generated, overrides previous mappings of that variable (effectively deletes them, acknowledging different binder)*)
+Definition rename_pseudo_bruijn (P : process) (avoid : list fin) : process := 
+  let fix ren p av mp := 
+    match p with
+      | p_var x => 
+          let fix maps_using xs x := 
+            match xs with 
+              | (from,to)::ys => if Nat.eqb from x then to else maps_using ys x
+              | [] => x
+            end 
+          in p_var (maps_using mp x)
+      | p_send p l e P' => p_send p l e (ren P' av mp)
+      | p_recv p lis => p_recv p (list_map (prod_map (fun x => x) (fun x => ren x av mp)) lis)
+      | p_ite e p1 p2 => p_ite e (ren p1 av mp) (ren p2 av mp)
+      | p_rec x P' => 
+          let fre := fresh_from_list av
+          in p_rec fre (ren P' (fre::av) ((x,fre)::mp))
+      | _ => p
+    end
+  in ren P (avoid ++ (fv P)) [].
+ 
+
+Compute rename_pseudo_bruijn recursive_mu [].
+Compute recursive_mu.
+
+Definition expr_eq_dec : forall (x y : expr), { x = y } + { x <> y }.
+Proof.
+decide equality.
+decide equality.
+decide equality. decide equality. decide equality. decide equality. decide equality. decide equality. decide equality.
+Defined.
+
+Definition balpha_equiv (P : process) (Q : process) : bool :=
+  let fix syntax_eq P1 P2 :=
+    match P1 with 
+    | p_var x =>
+        match P2 with 
+          | p_var y => (Nat.eqb x y)
+          | _ => false
+        end
+    | p_inact =>
+        match P2 with
+          | p_inact => true 
+          | _ => false
+        end 
+    | p_send p l e P' =>
+        match P2 with
+          | p_send q l' e' Q' => (eqb p q) && (Nat.eqb l l') && (expr_eq_dec e e') && (syntax_eq P' Q')
+          | _ => false 
+        end
+    | p_recv p lis =>
+        match P2 with
+          | p_recv q lis' => 
+            let fix all_true xs ys := 
+              match xs with
+                | (l,p')::xs' => 
+                  match ys with 
+                    | [] => false 
+                    | (l',q')::ys' => (Nat.eqb l l') && (syntax_eq p' q') && (all_true xs' ys')
+                  end
+                | [] => 
+                  match ys with
+                    | [] => true
+                    | _ => false
+                  end
+              end
+            in (eqb p q) && (all_true lis lis')
+          | _ => false
+        end
+    | p_ite e p1 p2 =>
+        match P2 with 
+          | p_ite e' q1 q2 => (expr_eq_dec e e') && (syntax_eq p1 q1) && (syntax_eq p2 q2)
+          | _ => false 
+        end
+    | p_rec x P' =>
+        match P2 with 
+          | p_rec y Q' => if Nat.eqb x y then syntax_eq P' Q' else false
+          | _ => false 
+        end
+   end
+  in syntax_eq (rename_pseudo_bruijn P (fv P ++ fv Q)) (rename_pseudo_bruijn Q (fv P ++ fv Q)). *)
+  
+  (* 
+Definition al1 := p_rec 0 (p_rec 1 (p_recv "Alice " [(1, p_var 0); (2, p_var 1)])).
+Definition al2 := p_rec 1 (p_rec 0 (p_recv "Alice " [(1, p_var 1); (2, p_var 0)])).
+Definition al3 := p_rec 20 (p_rec 13 (p_recv "Alice " [(1, p_var 20); (2, p_var 13)])).
+Definition al4 := p_rec 0 (p_rec 1 (p_recv "Alice " [(1, p_var 1); (2, p_var 1)])).
+
+Compute balpha_equiv al1 al2.
+Compute balpha_equiv al1 al4.
+Compute rename_pseudo_bruijn (p_rec 20 (p_rec 13 (p_var 20))) [].
+
+(* Example t : 2 <> 3.
+Proof.
+  simpl. easy. *)
+(*
+Lemma stronger_multi {X : Type} (R : relation X) : forall (x y z : X), multi R x y -> multi R y z -> multi R x z.
+Proof.
+  intros x y z.
+   *)
+  
+
+Example al1_al3 : alpha_multistep al1 al3. 
+Proof.
+  unfold al1, al3.
+  unfold alpha_multistep.
+  apply multi_step with 
+  (y := (p_rec 20 (p_rec 1 (p_recv "Alice " [(1, p_var 20); (2, p_var 1)])))).
+  apply a_recl. 
+  - unfold fresh_in. simpl. easy.
+  - unfold p_rename. unfold rename_force. simpl. easy.
+  
+  apply multi_step with 
+  (y := (p_rec 20 (p_rec 13 (p_recv "Alice " [(1, p_var 20); (2, p_var 13)])))).
+  apply a_rec2. apply a_recl. 
+  - unfold fresh_in. simpl. easy.
+  - unfold p_rename; unfold rename_force. simpl. easy.
+  
+  apply multi_refl.
+  
+Qed.
+
+Example al3_al2 : alpha_multistep al3 al2. 
+Proof.
+  unfold al3, al2.
+  unfold alpha_multistep.
+  apply multi_step with 
+  (y := (p_rec 1 (p_rec 13 (p_recv "Alice " [(1, p_var 1); (2, p_var 13)])))).
+  apply a_recl. 
+  - unfold fresh_in. simpl. easy.
+  - unfold p_rename. unfold rename_force. simpl. easy.
+  
+  apply multi_step with 
+  (y := (p_rec 1 (p_rec 0 (p_recv "Alice " [(1, p_var 1); (2, p_var 0)])))).
+  apply a_rec2. apply a_recl. 
+  - unfold fresh_in. simpl. easy.
+  - unfold p_rename; unfold rename_force. simpl. easy.
+  
+  apply multi_refl.
+  
+Qed.
+ *)
+  
+  
+  (* 
+Example al1_al2 : alpha_multistep al1 al2.
+Proof. 
+  unfold al1, al2.
+  apply transitive_multi with 
+  (y := al3).
+  apply al1_al3.
+  apply al3_al2.
+Qed. *)
